\documentclass{article}
\usepackage[english]{babel}
\usepackage[utf8]{inputenc}
\usepackage[OT4]{fontenc}
\usepackage{amsmath}
%\usepackage{dsfont}
\usepackage{graphicx}
\usepackage{amsthm}
\usepackage{amssymb}
%\usepackage[landscape,margin=1cm]{geometry}
\usepackage[a5paper]{geometry}
%\usepackage{fullpage}
\usepackage{colortbl}
\title{Reducing parasitic currents}
\author{\L{}ukasz \L{}aniewski-Wo\l{}\l{}k\footnote{llaniewski@meil.pw.edu.pl, C-CFD group, Warsaw University of Technology. http://c-cfd.meil.pw.edu.pl/}}

%\newcommand{\R}{\mathds{R}}
\newcommand{\pr}[1]{\frac{\partial}{\partial #1}}
\newcommand{\rr}[2]{\frac{\partial #1}{\partial #2}}
\newcommand{\ppr}[1]{\frac{\partial^2}{\partial #1^2}}
\newcommand{\prr}[2]{\frac{\partial^2}{\partial #1\partial #2}}
\newcommand{\rpr}[2]{\frac{\partial^2 #1}{\partial #2^2}}
\newcommand{\rrr}[3]{\frac{\partial^2 #1}{\partial #2\partial #3}}

\newcommand{\R}{\mathbb{R}}
\newcommand{\E}{\mathbb{E}}
\newcommand{\Var}{\text{Var}}
\newcommand{\eq}{\text{eq}}
\newcommand{\x}{\overline{x}}
\renewcommand{\t}{\overline{t}}
\newcommand{\f}{\tilde{f}}
\newcommand{\m}{\tilde{m}}
\renewcommand{\c}{\tilde{c}}
\begin{document}

\[\pr{t}f_i + e_i\nabla f_i = \Omega_i(f)\]


\[f_i(\x,\t) - f_i(x,t) = \frac{1}{2}\left(\Omega_i(f(\x,\t))+\Omega_i(f(x,t))\right)\]

\[f_i(\x,\t) - \frac{1}{2}\Omega_i(f(\x,\t)) = \frac{1}{2}\Omega_i(f(x,t)) + f_i(x,t)\]

\[\f_i(x,t) = f_i(x,t) - \frac{1}{2}\Omega_i(f(x,t))\]

\[\f_i(x,t) = \left(\text{Id} - \frac{1}{2}\Omega_i\right)(f(x,t))\]


\[\f_i(\x,\t) = \Omega_i(f(x,t)) + \f_i(x,t)\]

\[\f_i(\x,\t) = 2(f_i(x,t) - \f_i(x,t)) + \f_i(x,t)\]
\[\f_i(\x,\t) = 2f_i(x,t) - \f_i(x,t)\]

\[\f_i(\x,\t) = 2\left(\text{Id} - \frac{1}{2}\Omega_i\right)^{-1}\f_i(x,t) - \f_i(x,t)\]


\newpage

\newcommand{\C}{\mathcal{C}}
\[c = \C(f)\]
\[f = \C^{-1}(c)\]

\[\dot f_i = \rr{\C^{-1}_i}{c_j}(c)\dot c_j\]

\[\dot f_i = \rr{\C^{-1}_i}{c_j}(c)\gamma_j(c^\eq_j-c_j)\]

\[\pr{t}f_i + e_i\nabla f_i = \rr{\C^{-1}_i}{c_j}(c)\gamma_j(c^\eq_j-c_j)\]


\[f_i(\x,\t) - f_i(x,t) = \frac{1}{2}\left(\rr{\C^{-1}_i}{c_j}(c(\x,\t))\gamma_j(c^\eq_j(\x,\t)-c_j(\x,\t)) + \rr{\C^{-1}_i}{c_j}(c(x,t))\gamma_j(c^\eq_j(x,t)-c_j(x,t))\right)\]

\[f_i(\x,\t) - \frac{1}{2}\left(\rr{\C^{-1}_i}{c_j}(c(\x,\t))\gamma_j(c^\eq_j(\x,\t)-c_j(\x,\t))\right) = \frac{1}{2}\left( \rr{\C^{-1}_i}{c_j}(c(x,t))\gamma_j(c^\eq_j(x,t)-c_j(x,t))\right) + f_i(x,t)\]

\[\f_i = f_i - \frac{1}{2}\rr{\C^{-1}_i}{c_j}\gamma_j(c^\eq_j-\C_j(f))\]


\[\f_i = \rr{\C^{-1}_i}{c_j}\left(\left(\rr{\C^{-1}_i}{c_j}\right)^{-1}f_j + \frac{\gamma_j}{2}(\C_j(f) - c^\eq_j)\right)\]

\[\f_i = \rr{\C^{-1}_i}{c_j}\left(\left(\rr{\C^{-1}_i}{c_j}\right)^{-1}f_j + \frac{\gamma_j}{2}(\C_j(f) - c^\eq_j)\right)\]


\[\rr{\C_j}{f_i}\f_i + \frac{\gamma_j}{2}c^\eq_j = \rr{\C_j}{f_i}f_i + \frac{\gamma_j}{2}\C_j(f)\]



\[M_{ji}\f_i + \frac{\gamma_j}{2}m^\eq_j = M_{ji}f_i + \frac{\gamma_j}{2}M_{ji}f_i\]

\[M_{ji}\f_i + \frac{\gamma_j}{2}m^\eq_j = (1+\frac{\gamma_j}{2})M_{ji}f_i\]

\[\frac{2}{2+\gamma_j}M_{ji}\f_i + \frac{\gamma_j}{2+\gamma_j}m^\eq_j = M_{ji}f_i\]


\newpage

\[\left(\text{Id} - \frac{1}{2}\C\right)^{-1}\]

\newpage

\[c_j = \sum_k \Gamma^{\sigma_k}\prod_i m_{\sigma_i}\]
\[\rr{c_j}{m_n} = \sum_k 1_{n\in\sigma_k}\frac{1}{m_n}\Gamma^{\sigma_k}\prod_i m_{\sigma_i}\]

\[\sum_n\rr{c_j}{m_n}m_n = \sum_n\sum_k 1_{n\in\sigma_k}\Gamma^{\sigma_k}\prod_i m_{\sigma_i}\]

\[\sum_n\rr{c_j}{m_n}m_n = \sum_k |\sigma_k|\Gamma^{\sigma_k}\prod_i m_{\sigma_i}\]



\newpage


\[m_i = c_i + \Gamma_i(c_1,\ldots,c_{i-1})\]
\[\rr{m_i}{c_j} = \begin{cases}
0 & j > i\\
1 & j = 1\\
\rr{\Gamma_i}{c_j} & j < i
\end{cases}\]

\[c_i = m_i - \Gamma_i(c_1,\ldots,c_{i-1})\]


\[\m_i = m_i - \frac{1}{2}\rr{m_i}{c_j}\gamma_j(c^\eq_j-c_j)\]

\[\m_i = m_i - \frac{1}{2}\gamma_i(c^\eq_i-c_i) - \frac{1}{2}\rr{\Gamma_i}{c_j}\gamma_j(c^\eq_j-c_j)\]

\[\m_i = m_i - \frac{1}{2}\gamma_i(c^\eq_i-m_i + \Gamma_i(c_1,\ldots,c_{i-1})) - \frac{1}{2}\rr{\Gamma_i}{c_j}\gamma_j(c^\eq_j-c_j)\]


\[(1+\frac{\gamma_i}{2}) m_i = \m_i + \frac{1}{2}\gamma_i(c^\eq_i + \Gamma_i(c_1,\ldots,c_{i-1})) + \frac{1}{2}\rr{\Gamma_i}{c_j}\gamma_j(c^\eq_j-c_j)\]

\[m_i = \frac{2}{2+\gamma_i}\left(\m_i + \frac{1}{2}\gamma_i(c^\eq_i + \Gamma_i(c_1,\ldots,c_{i-1})) + \frac{1}{2}\rr{\Gamma_i}{c_j}\gamma_j(c^\eq_j-c_j)\right)\]


\[2m_i - \m_i = \frac{2-\gamma_i}{2+\gamma_i}\m_i + \frac{2}{2+\gamma_i}\left(\gamma_i(c^\eq_i + \Gamma_i(c_1,\ldots,c_{i-1})) + \rr{\Gamma_i}{c_j}\gamma_j(c^\eq_j-c_j)\right)\]


\[2m_i - \m_i = \omega_i\m_i + (1-\omega_i)(c^\eq_i + \Gamma_i(c_1,\ldots,c_{i-1})) + \frac{2}{2+\gamma_i}\rr{\Gamma_i}{c_j}\gamma_j(c^\eq_j-c_j)\]


\newpage

\[c_i = - \Gamma_i(c_1,\ldots,c_{i-1}) \]
\[m_i = \frac{2}{2+\gamma_i}\left(\m_i + \frac{1}{2}\gamma_i(c^\eq_i - c_i) + \frac{1}{2}\rr{\Gamma_i}{c_j}\gamma_j(c^\eq_j-c_j)\right)\]
\[c_i = c_i + m_i\]
\[m_i^\ast = 2m_i - \m_i\]
or:
\[c_i = \m_i - \Gamma_i(c_1,\ldots,c_{i-1}) \]
\[w = \frac{2}{2+\gamma_i}\left(\frac{1}{2}\gamma_i(c^\eq_i - c_i) + \frac{1}{2}\rr{\Gamma_i}{c_j}\gamma_j(c^\eq_j-c_j)\right)\]
\[c_i = c_i + w\]
\[m_i^\ast = \m_i + 2w\]
or:


\[c_i = - \Gamma_i(c_1,\ldots,c_{i-1}) \]
\[c_i = \frac{2}{2+\gamma_i}(\m_i + c_i) + \frac{\gamma_i}{2+\gamma_i}c^\eq_i + \frac{2}{2+\gamma_i}\frac{1}{2}\rr{\Gamma_i}{c_j}\gamma_j(c^\eq_j-c_j)\]
\[c_i = c_i + m_i\]
\[m_i^\ast = 2m_i - \m_i\]

\newpage

\[\m_i = m_i - \frac{1}{2}\rr{m_i}{c_j}\gamma_j(c^\eq_j-c_j)\]
\[h_j = \gamma_j(c^\eq_j-c_j)\]
\[w_i = \rr{m_i}{c_j}h_j\]
\[m_i = c_i + \sum_{jk}\Gamma^{ijk}c_jm_k\]
\[\rr{m_i}{c_p} = \delta_{ip} + \sum_{jk}\Gamma^{ijk}\left(\delta_{jp}m_k + c_j\rr{m_k}{c_p}\right)\]

\[w_i = \rr{m_i}{c_p}h_p = h_i + \sum_{jk}\Gamma^{ijk}\left(h_j m_k + c_j\rr{m_k}{c_p}h_p\right)\]

\[w_i = \rr{m_i}{c_p}h_p = h_i + \sum_{jk}\Gamma^{ijk}\left(h_j m_k + c_jw_k\right)\]

\[w_i = \gamma_i(c^\eq_i-c_i) + \sum_{jk}\Gamma^{ijk}\left(h_j m_k + c_jw_k\right)\]

\[w_i = \gamma_i(c^\eq_i-m_i + \sum_{jk}\Gamma^{ijk}c_jm_k) + \sum_{jk}\Gamma^{ijk}\left(h_j m_k + c_jw_k\right)\]

\[w_i = \gamma_i(c^\eq_i-\m_i-\frac{1}{2}w_i + \sum_{jk}\Gamma^{ijk}c_jm_k) + \sum_{jk}\Gamma^{ijk}\left(h_j m_k + c_jw_k\right)\]

\[(1+\frac{\gamma_i}{2})w_i = \gamma_i(c^\eq_i-\m_i + \sum_{jk}\Gamma^{ijk}c_jm_k) + \sum_{jk}\Gamma^{ijk}\left(h_j m_k + c_jw_k\right)\]


\[\m_i = m_i - \frac{1}{2}w_i\]
\[m_i^\ast = 2m_i - \m_i = \m_i+w_i\]
\[w_i = \m_i - m_i^\ast\]

\[\c_i = \m_i + \sum_{jk}\Gamma^{ijk}c_jm_k\]
\[m_i^\ast = \m_i+\frac{2}{2+\gamma_i}\left(\gamma_i(c^\eq_i-\c_i) + \sum_{jk}\Gamma^{ijk}\left(h_j m_k + c_jw_k\right)\right)\]

\newpage

A moment $m_i$ can be expressed as $c_i$ plus a combination of products of lower order moments and cumulants. We can thus say that:
\[m_i = c_i + \Gamma^{jk}_i c_j m_k\]
It can be also used the other way around:
\[c_i = m_i - \Gamma^{jk}_i c_j m_k\]
For a given vector $h_i$ we can define a vector $w_i$:
\[w_i = \rr{m_i}{c_j}h_j\]
This creates a recursive expression:
\begin{align*}w_i
&= \rr{m_i}{c_j}h_j =\\
&= \left(\delta_i^j + \Gamma^{ab}_i\left(\delta_a^j m_b + c_a\rr{m_b}{c_j}\right)\right)h_j=\\
&= h_i + \Gamma^{ab}_i \left(h_a m_b + c_a w_b\right)
\end{align*}
Now let us say that:
\[h_i = \Omega_i^j(c^\eq_j-c_j)\]

\end{document}

